---
layout: post
title: Proof of the Product Rule for Derivatives
categories: math
---


$$
\text{Let } h(x) = f(x)g(x). \text{ The derivative of } h(x) \text{ is given by:}
$$

$$
h’(x) = \lim_{\substack{\Delta x \to 0}} \frac{h(x + \Delta x) - h(x)}{\Delta x}
$$

$$
h’(x) = \lim_{\substack{\Delta x \to 0}} \frac{f(x + \Delta x)g(x + \Delta x) - f(x)g(x)}{\Delta x}
$$

<br>


$$
\text{Introduce and subtract } f(x + \Delta x)g(x):
$$

<br>


$$
h’(x) = \lim_{\substack{\Delta x \to 0}} \frac{f(x + \Delta x)g(x + \Delta x) - f(x + \Delta x)g(x) + f(x + \Delta x)g(x) - f(x)g(x)}{\Delta x}
$$

$$
\text{Separate into two limits:}
$$

$$
h’(x) = \lim_{\substack{\Delta x \to 0}} \left( \frac{f(x + \Delta x)g(x + \Delta x) - f(x + \Delta x)g(x)}{\Delta x} + \frac{f(x + \Delta x)g(x) - f(x)g(x)}{\Delta x} \right)
$$

$$
\text{Factorize common terms:}
$$

$$
h’(x) = \lim_{\substack{\Delta x \to 0}} \left( f(x + \Delta x) \frac{g(x + \Delta x) - g(x)}{\Delta x} + g(x) \frac{f(x + \Delta x) - f(x)}{\Delta x} \right)
$$

<br>


$$
\text{Apply the limits:}
$$

$$
h’(x) = f(x)g’(x) + g(x)f’(x)
$$

$$
\text{Therefore, the product rule is:}
$$

$$
(f(x)g(x))’ = f’(x)g(x) + f(x)g’(x)
$$

