---
layout: post
title: "Derivative of the tan(x) : Proof"
categories: math
---

$$
\tan'(x) = \lim_{\substack{h \to 0}} \frac{\tan(x + h) - \tan(x)}{h}
$$

$$
\text{Using the trigonometric identity for the tangent of a sum:}
$$

$$
\tan(x + h) = \frac{\tan(x) + \tan(h)}{1 - \tan(x)\tan(h)}
$$

<br>

$$
\tan'(x) = \lim_{\substack{h \to 0}} \frac{\frac{\tan(x) + \tan(h)}{1 - \tan(x)\tan(h)} - \tan(x)}{h}
$$

$$
\text{Combine the fractions:}
$$

$$
\tan'(x) = \lim_{\substack{h \to 0}} \frac{\tan(x) + \tan(h) - \tan(x)(1 - \tan(x)\tan(h))}{h(1 - \tan(x)\tan(h))}
$$

$$
\tan'(x) = \lim_{\substack{h \to 0}} \frac{\tan(x) + \tan(h) - \tan(x) + \tan(x)^2\tan(h)}{h(1 - \tan(x)\tan(h))}
$$

$$
\tan'(x) = \lim_{\substack{h \to 0}} \frac{\tan(h) + \tan(x)^2\tan(h)}{h(1 - \tan(x)\tan(h))}
$$

$$
\text{Factor out } \tan(h):
$$

$$
\tan'(x) = \lim_{\substack{h \to 0}} \frac{\tan(h)(1 + \tan(x)^2)}{h(1 - \tan(x)\tan(h))}
$$

<br>

$$
\text{Use the limit } \lim_{\substack{h \to 0}} \frac{\tan(h)}{h} = 1:
$$

$$
\tan'(x) = (1 + \tan(x)^2) \lim_{\substack{h \to 0}} \frac{\tan(h)}{h} \cdot \frac{1}{1 - \tan(x)\tan(h)}
$$

$$
\tan'(x) = (1 + \tan(x)^2) \cdot 1 \cdot \frac{1}{1 - 0}
$$

$$
\text{Simplify:}
$$

$$
\tan'(x) = 1 + \tan(x)^2
$$

$$
\text{Using the Pythagorean identity: } 1 + \tan(x)^2 = \sec(x)^2
$$

$$
\tan'(x) = \sec(x)^2
$$

$$
\text{So, the derivative of } \tan(x) \text{ is } \sec(x)^2.
$$
