---
layout: post
title:  "The differentiation of a fraction:proof"
categories: math

---

$$
\displaystyle \frac{d}{dx} \left( \frac{1}{g(x)} \right) = -\frac{g'(x)}{[g(x)]^2}
$$

$$
\text{Let } h(x) = \frac{1}{g(x)} \text{. We want to find } h'(x).
$$

$$
h'(x) = \lim_{\substack{\Delta x \to 0}} \displaystyle \frac{h(x + \Delta x) - h(x)}{\Delta x}
$$

$$
= \lim_{\substack{\Delta x \to 0}} \displaystyle \frac{\frac{1}{g(x + \Delta x)} - \frac{1}{g(x)}}{\Delta x}
$$

$$
= \lim_{\substack{\Delta x \to 0}} \displaystyle \frac{g(x) - g(x + \Delta x)}{g(x)g(x + \Delta x)\Delta x}
$$

$$
= -\lim_{\substack{\Delta x \to 0}} \displaystyle \frac{g(x + \Delta x) - g(x)}{g(x)g(x + \Delta x)\Delta x}
$$

$$
= -\frac{\lim_{\substack{\Delta x \to 0}} \displaystyle \frac{g(x + \Delta x) - g(x)}{\Delta x}}{g(x)\lim_{\substack{\Delta x \to 0}}g(x + \Delta x)}
$$

$$
= -\frac{g'(x)}{g(x)g(x)}
$$

$$
= -\frac{g'(x)}{[g(x)]^2}
$$
