---
layout: post
title: "Derivative of the sigmoid function : Proof"
categories: math

---
$$
\text{Given: }
$$

$$
\frac{d}{dx} \left( \frac{1}{1+e^{-x}} \right)
$$

$$
\text{Apply the quotient rule: }
$$

$$
= - \frac{(1+e^{-x})'}{(1+e^{-x})^2}
$$

$$
\text{Differentiate the numerator: }
$$

$$
= - \frac{0 - e^{-x}}{(1+e^{-x})^2}
$$

$$
\text{Simplify: }
$$

$$
= \frac{e^{-x}}{(1+e^{-x})^2}
$$

$$
\text{Recognize the sigmoid function: } \frac{1}{1+e^{-x}} \text{ is } \text{sig}(x)
$$

$$
\text{Substitute: }
$$

$$
= \text{sig}(x) \cdot \left( 1 - \text{sig}(x) \right)
$$

$$
\text{For the natural logarithm derivative: }
$$

$$
(\ln(x))' = \lim_{h \to 0} \frac{\ln(x+h) - \ln(x)}{h}
$$

$$
\text{Using the properties of logarithms: }
$$

$$
= \lim_{h \to 0} \frac{\ln\left(\frac{x+h}{x}\right)}{h}
$$
