---
layout: post
title: "Derivative of the Natural Logarithm : Proof"
categories: math

---

<br>
<br>


## Natural log

{% raw %}
$$
(\ln(x))' = \lim_{h \to 0} \frac{\ln(x+h) - \ln(x)}{h}
$$

$$
= \lim_{h \to 0} \frac{\ln\left(\frac{x+h}{x}\right)}{h}
$$

$$
Substitute : u=x+h
$$

$$
= \lim_{u \to x} \frac{\ln\left(\frac{u}{x}\right)}{u - x}
$$

$$
= \lim_{u \to x} \frac{\ln\left(1 + \frac{u - x}{x}\right)}{u - x}
$$

$$
Substitute :  v = \frac{u - x}{x}
$$

$$
= \lim_{v \to 0} \frac{\ln(1 + v)}{xv}
$$

$$
= \frac{1}{x} \times \lim_{v \to 0} v
$$

$$
= \frac{1}{x} \times 1
$$

$$
(\ln(x))' = \frac{1}{x}
$$
{% endraw %}



<br>
<br>

##  log

$$
\log_b(x) = \frac{\ln(x)}{\ln(b)}
$$

$$
\frac{d}{dx} \log_b(x) = \frac{d}{dx} \left( \frac{\ln(x)}{\ln(b)} \right)
$$

$$
= \frac{1}{\ln(b)} \cdot \frac{d}{dx} \ln(x)
$$

$$
= \frac{1}{\ln(b)} \cdot \frac{1}{x}
$$

$$
\frac{d}{dx} \log_b(x) = \frac{1}{x \ln(b)}
$$