---
layout: post
title: "Derivative of the chain law : Proof"
categories: math

---


$$
\frac{d}{dx}f(g(x)) =  \lim_{\substack{\Delta x \to 0}} \displaystyle \frac{f(g(x + \Delta x)) - f(g(x))}{\Delta x}
$$




$$
Let :  u = g(x) \; then \;  (f \circ g)(x) = f(u),

$$

$$
 then:
\frac{d}{dx}f(g(x)) = \lim_{\substack{\Delta x \to 0}} \displaystyle \frac{f(g(x + \Delta x)) - f(g(x))}{\Delta x}
$$

$$
\lim_{\substack{\Delta x \to 0}} \displaystyle \frac{f(u + \Delta u) - f(u)}{\Delta x}
$$

$$
\lim_{\substack{\Delta x \to 0}} \displaystyle \frac{f(u + \Delta u) - f(u)}{\Delta u} \cdot \frac{\Delta u}{\Delta x}
$$

$$
\left(\lim_{\substack{\Delta u \to 0}} \displaystyle \frac{f(u + \Delta u) - f(u)}{\Delta u}\right) \cdot \left(\lim_{\substack{\Delta x \to 0}} \displaystyle \frac{\Delta u}{\Delta x}\right)
$$

$$
\frac{df}{du} \cdot \frac{du}{dx}
$$

$$
\frac{d}{dx}f(g(x)) = \frac{df}{du} \cdot \frac{du}{dx}
$$

$$
u = g(x) 
$$

$$
\frac{d}{dx}f(g(x)) = \frac{df}{dg} \cdot \frac{dg}{dx}
$$