---
layout: post
title: "Derivative of the natural constant : Proof"
categories: math
---

$$
f'(x) = \lim_{\substack{h \to 0}} \frac{f(x + h) - f(x)}{h}
$$

$$
f'(x) = \lim_{\substack{h \to 0}} \frac{e^{x + h} - e^x}{h}
$$

$$
f'(x) = \lim_{\substack{h \to 0}} \frac{e^x \cdot e^h - e^x}{h}
$$

$$
f'(x) = \lim_{\substack{h \to 0}} e^x \cdot \frac{e^h - 1}{h}
$$

$$
\text{Apply the L'Hôpital's rule:}
$$

$$
\lim_{\substack{h \to 0}} \frac{e^h - 1}{h} = 1
$$

$$
f'(x) = e^x
$$

<br>
<br>
<br>

$$
\text{ *** Applying L'Hôpital's rule part:}
$$

$$
\lim_{\substack{h \to 0}} \frac{e^h - 1}{h} = \lim_{\substack{h \to 0}} \frac{(e^h)'}{(h)'}
$$

$$
\text{Where:}
$$

$$
\begin{cases}
(e^h)' = e^h \\
(h)' = 1
\end{cases}
$$

$$
\text{So, the limit becomes:}
$$

$$
\lim_{\substack{h \to 0}} \frac{e^h}{1} = \lim_{\substack{h \to 0}} e^h = e^0 = 1
$$
