---
layout: post
title: Proof of the Power Rule for Derivatives
categories: math
---

$$
\text{Let } f(x) = x^n. \text{ The derivative of } f(x) \text{ is given by:}
$$

$$
f’(x) = \lim_{\substack{h \to 0}} \frac{f(x + h) - f(x)}{h}
$$

$$
f’(x) = \lim_{\substack{h \to 0}} \frac{(x + h)^n - x^n}{h}
$$

<br>

$$
\text{Expand } (x + h)^n \text{ using the Binomial Theorem:}
$$

$$
(x + h)^n = x^n + nx^{n-1}h + \frac{n(n-1)}{2}x^{n-2}h^2 + \cdots + h^n
$$

<br>

$$
\text{Substitute into the limit:}
$$

$$
f’(x) = \lim_{\substack{h \to 0}} \frac{x^n + nx^{n-1}h + \frac{n(n-1)}{2}x^{n-2}h^2 + \cdots + h^n - x^n}{h}
$$

$$
\text{Cancel out the } x^n \text{ terms:}
$$

$$
f’(x) = \lim_{\substack{h \to 0}} \frac{nx^{n-1}h + \frac{n(n-1)}{2}x^{n-2}h^2 + \cdots + h^n}{h}
$$

<br>

$$
\text{Factor out } h \text{ from the numerator:}
$$

$$
f’(x) = \lim_{\substack{h \to 0}} \frac{h \left(nx^{n-1} + \frac{n(n-1)}{2}x^{n-2}h + \cdots + h^{n-1}\right)}{h}
$$

$$
\text{Cancel } h \text{ in the numerator and denominator:}
$$

$$
f’(x) = \lim_{\substack{h \to 0}} \left(nx^{n-1} + \frac{n(n-1)}{2}x^{n-2}h + \cdots + h^{n-1}\right)
$$

<br>

$$
\text{Apply the limit as } h \to 0:
$$

$$
f’(x) = nx^{n-1}
$$

$$
\text{Therefore, the power rule is:}
$$

$$
\frac{d}{dx} x^n = nx^{n-1}
$$
